\documentclass{article}
\usepackage[utf8]{inputenc}
\usepackage{amsmath,amsthm,amsfonts}
\begin{document}
\section*{Induction Exercise 2}
Prove that
\[
	\sum_{i=0}^{n} i^3 = 1^3 + 2^3 + 3^3 + ... + n^3 = (1+2+3+...+n)^3
\]
\begin{proof}
	If $n=1$, then
	\[
		\sum_{i=0}^{1} i^3 = 1 = (1)^3.
	\]
	Thus the statement is true for $n=1$.
	\newline\newline
	Now assuming that
	\[
		\sum_{i=0}^{k} i^3 = (1+2+3+...+k)^3
	\]
	we find that 
	\begin{align*}
		\sum_{i=0}^{k+1} i^3 & = \sum_{i=0}^{k} i^3 + (k+1)^3\\
				     & = (1+2+3+...+k)^3 + (k+1)^3 \\
				     & = \left( \frac{k(k+1)}{2} \right)^3 + (k+1)^3 \\
				     & = \left( \left( \frac{k(k+1)}{2} \right) + (k+1) \right)^3 \\
				     & = \left( \frac{k(k+1)+2(k+1)}{2} \right)^3 \\
				     & = \left( \frac{(k+1)(k+2)}{2} \right)^3 \\
				     & = \left( \frac{(k+1)((k+1)+1)}{2} \right)^3 \\
				     & = (1+2+3+...+(k+1))^3.
	\end{align*}
	Hence by the priniciple of mathematical induction we have established that the statement is true for all $n \in \mathbb{N}$.
\end{proof}
\end{document}
