\documentclass{article}
\usepackage[utf8]{inputenc}
\usepackage{amsmath,amsthm,amsfonts}
\begin{document}
\section*{Induction Exercise 4}
Prove that
\[
	\sum_{i=0}^{n} i(i+1) = 1\cdot2 + 2\cdot3 + 3\cdot4 + ... + n(n+1) = \frac{n(n+1)(n+2)}{3}
\]
\begin{proof}
	If $n=1$, then
	\[
		\sum_{i=0}^{1} i(i+1) = 2 = \frac{1(2)(3)}{3}.
	\]
	Thus the statement is true for $n=1$.
	\newline\newline
	Now assuming that
	\[
		\sum_{i=0}^{k} i(i+1) = \frac{k(k+1)(k+2)}{3}
	\]
	we find that 
	\begin{align*}
		\sum_{i=0}^{k+1} i(i+1) & = \left( \sum_{i=0}^{k} i(i+1) \right) + (k+1)((k+1)+1) \\
				        & = \frac{k(k+1)(k+2)}{3} + (k+1)(k+2) \\
				        & = \frac{k(k+1)(k+2) + 3(k+1)(k+2)}{3} \\
				        & = \frac{(k+1)(k+2)(k+3)}{3} \\
				        & = \frac{(k+1)((k+1)+1)((k+1)+2)}{3}.
	\end{align*}
	Hence by the priniciple of mathematical induction we have established that the statement is true for all $n \in \mathbb{N}$.
\end{proof}
\end{document}
