\documentclass{article}
\usepackage[utf8]{inputenc}
\usepackage{amsmath,amsthm}

\title{Number Theory Exercises}
\author{Aiden Taylor}
\date{August 2022}

\begin{document}

%\maketitle

\section{Induction Exercises}
\subsection{}
Prove that
\[
	\sum_{i=0}^{n} i^2 = 1^2 + 2^2 + 3^2 + ... + n^2 = \frac{n(n+1)(2n+1)}{6} (*)
\]
\begin{proof}
	If $n=1$, then
	\[
		\sum_{i=0}^{1} i^2 = 1 = \frac{1(1+1)(2+1)}{6}
	\]
	thus $(*)$ is true for $n=1$.
	\newline\newline
	Now assume $(*)$ is true for $n = k$, such that
	\[
		\sum_{i=0}^{k} i^2 = \frac{k(k+1)(2k+1)}{6}
	\]
	We then need to prove that $(*)$ is true for $n=k+1$. Adding $(k+1)^2$ to both sides of our assumption gets 
	\begin{align*}
		\sum_{i=0}^{k+1} i^2 & = \frac{k(k+1)(2k+1)}{6} + (k+1)^2 \\
				     & = (k+1) \left[ \frac{k(2k+1)}{6} + (k+1) \right] \\
				     & = (k+1) \left[ \frac{k(2k+1) + 6(k+1)}{6} \right] \\
				     & = (k+1) \left[ \frac{2k^2 + k + 6k + 6}{6} \right] \\
				     & = (k+1) \left[ \frac{2k^2 + 4k + 3k + 6}{6} \right] \\
				     & = (k+1) \left[ \frac{2k(k+2) + 3(k+2)}{6} \right] \\
				     & = (k+1) \left[ \frac{(k+2)(2k+3)}{6} \right] \\
				     & = \frac{(k+1)(k+2)(2k+3)}{6} \\
				     & = \frac{(k+1)((k+1)+1)(2(k+1)+1)}{6}
	\end{align*}
	where the last equation is the same as $(*)$ with $n=k+1$. Hence by the priniciple of mathematical induction $(*)$ is true for all $n \in \mathbf{N}$.
\end{proof}
\end{document}
