\documentclass{article}
\usepackage[utf8]{inputenc}
\usepackage{amsmath,amsthm,amsfonts}
\begin{document}
\section*{Induction Exercise 5}
Prove that
\[
	\sum_{i=1}^{n} (2i-1) = 1 + 3 + 5 + ... + (2n-1) = n^2.
\]
\begin{proof}
	If $n=1$, then
	\[
		\sum_{i=1}^{1} (2i-1) = 1 = 1^2.
	\]
	Thus the statement is true for $n=1$.
	\newline\newline
	Now assuming that
	\[
		\sum_{i=1}^{k} (2i-1) = k^2
	\]
	we find that 
	\begin{align*}
		\sum_{i=1}^{k+1} (2i-1) & = \left( \sum_{i=1}^{k} (2i-1) \right) + \left(2(k+1)-1\right) \\
				        & = k^2 + 2(k+1) - 1 \\
				        & = k^2 + 2k + 1 \\
				        & = (k+1)(k+1) \\
				        & = (k+1)^2.
	\end{align*}
	Hence by the priniciple of mathematical induction we have established that the statement is true for all $n \in \mathbb{N}$.
\end{proof}
\end{document}
